theories/Relations.v
@@ -28,26 +28,313 @@ Proof.
     destruct (lift_tm_max _ _ _ _ i i0 H0 H9).
     destruct (lift_eq_max _ _ _ _ _ _ i i0 H2 H10).
     destruct (lift_eq_max _ _ _ _ _ _ i i0 H3 H12).
-    econstructor;mauto.
-    -- eapply (ctxeq_eq _ _ _ _ _ (ctx_eq_sym _ _ H)).
-       mauto.
-    -- eapply (ctxeq_eq _ _ _ _ _ H7).
-       mauto.    
+    econstructor;mauto. 
 Qed.
+
+Definition rel_tm (Γ : Ctx) (T : Typ) (t : exp) : Prop := (wf_term Γ t T).
+Definition rel_sb (Γ Δ: Ctx) (σ : Sb) : Prop := (wf_sb Γ σ Δ).
+
+Definition term_eq (Γ : Ctx) (T : Typ) (t t' : exp) : Prop := (wf_term_eq Γ t t' T).
+Definition sb_eq (Γ Δ : Ctx) (σ σ' : Sb) : Prop := (wf_sub_eq Γ σ σ' Δ).
+
+
+
+
+Lemma wf_to_term_eq (Γ : Ctx) (T : Typ) (t t' : exp) : wf_term_eq Γ t t' T -> term_eq Γ T t t'.
+Proof.
+  intros;auto.
+Qed.  
+
+Lemma wf_to_sb_eq (Γ Δ : Ctx) (σ σ' : Sb) : wf_sub_eq Γ σ σ' Δ -> sb_eq Γ Δ σ σ'.
+Proof.
+  intros;auto.
+Qed.  
+
+Lemma term_eq_to_wf (Γ : Ctx) (T : Typ) (t t' : exp) : term_eq Γ T t t'-> wf_term_eq Γ t t' T.
+Proof.
+  intros;auto.
+Qed.  
+  
+Lemma sb_eq_to_wf (Γ Δ : Ctx) (σ σ' : Sb) : sb_eq Γ Δ σ σ' -> wf_sub_eq Γ σ σ' Δ .
+Proof.
+  intros;auto.
+Qed.
+
+Lemma rel_tm_to_wf_term (Γ : Ctx) (T : Typ) (t : exp) : rel_tm Γ T t -> Γ ⊢ t : T .
+Proof.
+  auto.
+Qed.
+
+Lemma rel_sb_to_wf_sub (Γ Δ : Ctx) (σ : Sb) : rel_sb Γ Δ σ -> Γ ⊢s σ : Δ.
+Proof.
+  auto.
+Qed.
+
+Lemma wf_term_to_rel_tm (Γ : Ctx) (T : Typ) (t : exp) : Γ ⊢ t : T -> rel_tm Γ T t.
+Proof.
+  auto.
+Qed.
+
+Lemma wf_sb_to_rel_sb (Γ Δ : Ctx) (σ : Sb) : Γ ⊢s σ : Δ -> rel_sb Γ Δ σ.
+Proof.
+  auto.
+Qed.
+  
+Lemma tm_symmetry (Γ : Ctx) (T : Typ) (t t' : exp) : term_eq Γ T t t' -> term_eq Γ T t' t.
+Proof.
+  intros.
+  auto using term_eq_to_wf,wf_to_term_eq,wf_eq_sym.
+Qed.  
+
+Lemma tm_transitivity (Γ : Ctx) (T : Typ) (t t' t'' : exp) :  term_eq Γ T t t' -> term_eq Γ T t' t'' ->  term_eq Γ T t t''.
+Proof.
+  intros.
+  eauto using term_eq_to_wf,wf_to_term_eq,wf_eq_trans.
+Qed.
+
+Lemma sb_symmetry (Γ Δ: Ctx) (σ σ' : Sb) : sb_eq Γ Δ σ σ' -> sb_eq Γ Δ σ' σ.
+Proof.
+  intros.
+  auto using sb_eq_to_wf,wf_to_sb_eq,wf_sub_eq_sym.
+Qed.  
+
+Lemma sb_transitivity (Γ Δ: Ctx) (σ σ' σ'' : Sb) :  sb_eq Γ Δ σ σ' -> sb_eq Γ Δ σ' σ'' ->  sb_eq Γ Δ σ σ''.
+Proof.
+  intros.
+  eauto using sb_eq_to_wf,wf_to_sb_eq,wf_sub_eq_trans.
+Qed.  
 
 
 
 Add Parametric Relation : (Ctx) (wf_ctx_eq)
     symmetry proved by ctx_eq_sym
     transitivity proved by ctx_eq_trans
-    as ctx_eq.
+    as ctx_eq_rel.
 
-Add Parametric Relation (Γ : Ctx) (T : Typ) : (exp) (λ t t',wf_term_eq Γ t t' T)
-    symmetry proved by (λ t t',wf_eq_sym Γ t t' T)
-    transitivity proved by (λ t t' t'', wf_eq_trans Γ t t' T t'')
-    as tm_eq.                                                
+Add Parametric Relation (Γ : Ctx) (T : Typ) : (exp) (term_eq Γ T)
+    symmetry proved by (tm_symmetry Γ T)
+    transitivity proved by (tm_transitivity Γ T)
+    as tm_eq_rel.                                                
 
-Add Parametric Relation (Γ Δ : Ctx) : (Sb) (λ σ τ, wf_sub_eq Γ σ τ Δ)
-    symmetry proved by (λ σ τ, wf_sub_eq_sym Γ σ τ Δ)
-    transitivity proved by (λ σ τ ρ, wf_sub_eq_trans Γ σ τ Δ ρ)
-    as sb_eq.
+Add Parametric Relation (Γ Δ : Ctx) : (Sb) (sb_eq Γ Δ)
+    symmetry proved by (sb_symmetry Γ Δ)
+    transitivity proved by (sb_transitivity Γ Δ)
+    as sb_eq_rel.
+
+
+Ltac convert_hypotheses_to_relational :=
+  let rec convert:=
+    match goal with
+    | [H : (?Γ ⊢ ?t ≈ ?t' : ?T) |- _] => (apply wf_to_term_eq in H);convert
+    | [H : (?Γ ⊢s ?σ ≈ ?σ' : ?Δ) |- _] => (apply wf_to_sb_eq in H);convert
+    | [H : (?Γ ⊢ ?t : ?T) |- _] => (apply wf_term_to_rel_tm in H);convert
+    | [H : (?Γ ⊢s ?σ : ?Δ) |- _] => (apply wf_sb_to_rel_sb in H);convert
+    | [H : _ |- _ ] => idtac
+    end
+  in convert
+.
+
+Ltac convert_hypotheses_to_term := let rec convert:=
+    match goal with
+    | [H : (term_eq ?Γ ?T ?t ?t') |- _] => (apply term_eq_to_wf in H);convert
+    | [H : (sb_eq ?Γ ?Δ ?σ ?σ') |- _] => (apply sb_eq_to_wf in H);convert
+    | [H : (rel_tm ?Γ ?T ?t) |- _] => (apply rel_tm_to_wf_term in H);convert
+    | [H : (rel_sb ?Γ ?Δ ?t) |- _] => (apply rel_sb_to_wf_sub in H);convert
+    | [H : _ |- _ ] => idtac
+    end
+  in convert
+.
+
+
+Ltac convert_to_relational :=
+  (try eapply term_eq_to_wf);
+  (try eapply rel_tm_to_wf_term);
+  (try eapply rel_sb_to_wf_sub);
+  (try eapply sb_eq_to_wf);
+  convert_hypotheses_to_relational.
+
+Ltac convert_from_relational :=
+  (try eapply wf_to_term_eq);
+  (try eapply wf_term_to_rel_tm);
+  (try eapply wf_sb_to_rel_sb);
+  (try eapply wf_to_sb_eq);
+  convert_hypotheses_to_term.
+
+Add Parametric Morphism (Γ : Ctx) (i : nat) : (term_eq Γ)
+    with signature (term_eq Γ (typ i)) ==> (eq) ==> (eq) ==> (iff)
+      as eq_mor.
+Proof.
+  intros.
+  split;intros;convert_from_relational;mauto.
+Qed.
+
+Add Parametric Morphism (Γ : Ctx) (i : nat) : (rel_tm Γ) with signature (term_eq Γ (typ i)) ==> (eq) ==> (iff) as tm_mor.
+Proof.
+  intros.
+  split;intros;convert_from_relational;mauto.
+Qed.  
+
+Add Parametric Morphism : (wf_term)
+    with signature (wf_ctx_eq) ==> (eq) ==> (eq) ==> (iff) as ctx_tm_mor.
+Proof.
+  intros.
+  split;intros;mauto.
+Qed.
+
+Add Parametric Morphism : (wf_term_eq) with signature (wf_ctx_eq) ==> (eq) ==> (eq) ==>(eq) ==> (iff) as ctx_eq_mor.                        
+Proof.
+  intros.
+  split;intros;mauto.
+Qed.
+
+Add Parametric Morphism : (wf_sb) with signature (wf_ctx_eq) ==> (eq) ==> (eq) ==> (iff) as ctx_sb_mor1.                        
+Proof.  
+  intros.
+  split;intros;mauto.
+Qed.
+
+Add Parametric Morphism : (wf_sb) with signature (wf_ctx_eq) ==> (eq) ==> (eq) ==> (iff) as ctx_sb_mor2.                        
+Proof.  
+  intros.
+  split;intros;mauto.
+Qed.
+
+Add Parametric Morphism : (wf_sub_eq) with signature (wf_ctx_eq) ==> (eq) ==> (eq) ==> (eq)==> (iff) as ctx_sb_eq_mor1.
+Proof.  
+  intros.
+  split;intros;mauto.
+Qed.
+
+Add Parametric Morphism : (wf_sub_eq) with signature (wf_ctx_eq) ==> (eq) ==> (eq) ==> (eq)==> (iff) as ctx_sb_eq_mor2.
+Proof.  
+  intros.
+  split;intros;mauto.
+Qed.
+
+Check a_.
+
+Generalizable All Variables.
+
+
+Lemma rew_tm_nat_sub : `(rel_sb Γ Δ σ -> term_eq Γ (typ i) (ℕ ⟦ σ ⟧) (ℕ)).
+Proof.
+  intros.
+  convert_from_relational;mauto.
+Qed.
+
+Lemma rew_tm_typ_sub : `(rel_sb Γ Δ σ ->term_eq Γ (typ (i+1)) (typ i ⟦ σ ⟧) (typ i)).
+Proof.
+  intros.
+  convert_from_relational;mauto.
+Qed.
+
+
+Lemma rew_tm_pi_sub : `(rel_sb Γ Δ σ -> rel_tm Δ (typ i) T' -> rel_tm (T' :: Δ) (typ i) T -> term_eq Γ (typ i) ((Π T' T) ⟦ σ ⟧)  (Π (T' ⟦ σ ⟧) (T ⟦var_wk σ ⟧))).
+Proof.
+  intros.
+  convert_from_relational;mauto.
+Qed.
+
+
+Lemma rew_tm_zero_sub : `(rel_sb Γ Δ σ -> term_eq Γ (ℕ) (a_zero ⟦ σ ⟧) (a_zero)).
+Proof.
+  intros.
+  convert_from_relational;mauto.
+Qed.
+
+Lemma rew_tm_succ_sub : `(rel_sb Γ Δ σ -> rel_tm Δ ℕ t -> term_eq Γ (ℕ) ((a_succ t) ⟦ σ ⟧) (a_succ (t ⟦ σ ⟧))).
+Proof.
+  intros.
+  convert_from_relational;mauto.
+Qed.
+
+Lemma rew_tm_sub_cong : `(term_eq Δ T t t' -> sb_eq Γ Δ σ σ' -> term_eq Γ (T ⟦ σ ⟧) (t ⟦ σ ⟧) (t' ⟦ σ ⟧)).
+Proof.
+  intros.
+  convert_from_relational;mauto.
+Qed.
+
+Lemma rew_tm_sub_comp : `(rel_sb Γ Γ' τ -> rel_sb Γ' Γ'' σ -> rel_tm Γ'' T t -> term_eq Γ (T ⟦ (σ ∙ τ) ⟧) (t ⟦ σ ∙ τ ⟧) ((t ⟦ σ ⟧) ⟦ τ ⟧)).
+Proof.
+  intros.
+  convert_from_relational;mauto.
+Qed.
+
+Lemma rew_tm_conv : `(term_eq Γ T t t' -> term_eq Γ (typ i) T T' -> term_eq Γ T' t t').
+Proof.
+  intros.
+  convert_from_relational;mauto.
+Qed.
+
+Lemma rew_sb_comp_cong : `(sb_eq Γ Γ' τ τ' -> sb_eq Γ' Γ'' σ σ' -> sb_eq Γ Γ'' (σ ∙ τ) (σ' ∙ τ')).
+Proof.
+  intros.
+  convert_from_relational;mauto.
+Qed.
+
+Lemma rew_sb_ext_cong : `(sb_eq Γ Δ σ σ' -> rel_tm Δ (typ i) T -> term_eq Γ (T ⟦ σ ⟧) t t' -> sb_eq Γ (T :: Δ) (σ ,, t) (σ ,, t')).
+Proof.
+  intros.
+  convert_from_relational;mauto.
+Qed.
+
+Lemma rew_sb_eq_id_r : `(rel_sb Γ Δ σ -> sb_eq Γ Δ (a_id ∙ σ) (σ)).
+Proof.
+  intros.
+  convert_from_relational;mauto.
+Qed.  
+
+Lemma rew_sb_eq_id_l : `(rel_sb Γ Δ σ -> sb_eq Γ Δ (σ ∙ a_id) (σ)).
+Proof.
+  intros.
+  convert_from_relational;mauto.
+Qed.
+
+Lemma rew_sb_comp_assoc : `(rel_sb Γ' Γ σ -> rel_sb Γ'' Γ' σ' -> rel_sb Γ''' Γ'' σ'' -> sb_eq Γ''' Γ ((σ ∙ σ') ∙ σ'') (σ ∙ (σ' ∙ σ''))).
+Proof.
+  intros.
+  convert_from_relational;mauto.
+Qed.       
+
+Lemma rew_sb_ext_comp : `(rel_sb Γ' Γ'' σ -> rel_tm Γ'' (typ i) T -> rel_tm Γ' (T ⟦ σ ⟧) (t) -> rel_sb Γ Γ' τ -> sb_eq Γ (T :: Γ'') ((σ ,, t) ∙ τ) ((σ ∙ τ) ,, (a_sub t τ))).
+Proof.
+  intros.
+  convert_from_relational;mauto.
+Qed.  
+
+Lemma rew_sb_p_ext : `(rel_sb Γ' Γ σ -> rel_tm Γ (typ i) T -> rel_tm Γ' (T ⟦ σ ⟧) t -> sb_eq Γ' Γ (sb_proj (σ ,, t)) σ).
+Proof.
+  intros.
+  convert_from_relational;mauto.
+Qed.    
+
+Lemma rew_sb_ext : `(rel_sb Γ' (T :: Γ) σ -> sb_eq Γ' (T :: Γ) σ (sb_proj σ ,, (a_var 0 ⟦ σ ⟧))). 
+Proof.
+  intros.
+  convert_from_relational;mauto.
+Qed. 
+
+(*Rewrite rules for types*)
+#[export]
+Hint Rewrite rew_tm_nat_sub rew_tm_pi_sub rew_tm_typ_sub rew_tm_conv using mauto : mcltt_types.
+(*Rewrite rules for terms*)
+#[export]
+Hint Rewrite rew_tm_sub_comp rew_tm_sub_cong rew_tm_succ_sub rew_tm_zero_sub using mauto: mcltt_terms.
+(*Rewrite rules for extension subs*)
+#[export]
+Hint Rewrite rew_sb_ext rew_sb_ext_comp rew_sb_ext_cong rew_sb_p_ext using mauto : mcltt_sub_ext. 
+(*Rewrite rules for substition algebra*) 
+#[export]
+Hint Rewrite rew_sb_comp_assoc rew_sb_comp_cong rew_sb_eq_id_l rew_sb_eq_id_r using mauto : mcltt_sub_alg.
+
+
+Lemma test (Γ : Ctx) : ⊢ Γ -> Γ ⊢ a_zero ⟦ a_id ∙ a_id ⟧ ≈ a_zero : ℕ.
+Proof.
+  intro.
+  convert_to_relational.
+  autorewrite with mcltt.
+  
+  eapply tm_eq_refl;mauto.
+  eapply wf_sb_to_rel_sb.
+  mauto.
+Qed.  
