theories/Syntax.v
@@ -1,6 +1,9 @@
 Require Import String.
 Require Import List.
 
+Declare Scope mcltt.
+Open Scope mcltt.
+
 (* CST term *)
 Module Cst.
 Inductive obj : Set :=
@@ -11,6 +14,7 @@ Inductive obj : Set :=
   | app : obj -> obj -> obj
   | fn : string -> obj -> obj -> obj
   | pi : string -> obj -> obj -> obj
+  | rec :  obj -> obj -> obj -> obj -> obj                           
   | var : string -> obj.
 End Cst.
 
@@ -19,6 +23,7 @@ Inductive exp : Set :=
   (* Natural numbers *)
   | a_zero : exp
   | a_succ : exp -> exp
+  | a_rec : exp -> exp -> exp -> exp -> exp                 
   (* Type constructors *)
   | a_nat : exp
   | a_typ : nat -> exp
@@ -36,8 +41,8 @@ with subst : Set :=
   | a_extend : subst -> exp -> subst.
 
 (* Some convenient infix notations *)
-Infix "∙" := a_compose (at level 70).
-Infix ",," := a_extend (at level 80).
+Infix "∙" := a_compose (at level 70) : mcltt.
+Infix ",," := a_extend (at level 80) : mcltt.
 
 
 Notation Ctx := (list exp).
@@ -47,3 +52,8 @@ Notation typ := a_typ.
 Notation ℕ := a_nat.
 Notation 𝝺 := a_fn.
 Notation Π := a_pi.
+Notation "x ⟦ σ ⟧" := (a_sub x σ) (at level 90, σ at next level) : mcltt.
+Notation "'var_wk' σ" := (σ ∙ a_weaken ,, a_var 0) (at level 70, σ at next level) : mcltt.
+Notation "x ⟦| σ ⟧" := (a_sub x (a_id,,σ)) (at level 90, σ at next level) : mcltt.
+Notation "'sb_proj' σ" := (a_weaken ∙ σ) (at level 70, σ at next level) : mcltt.
+Notation "M $ N" := (a_app M N) (at level 80, N at next level) : mcltt.
