theories/CtxEquiv.v
@@ -4,6 +4,8 @@ Require Import Mcltt.System.
 Require Import Mcltt.CtxEqLemmas.
 Require Import Mcltt.LibTactics.
 
+Open Scope mcltt.
+
 Lemma ctxeq_tm (Γ Δ : Ctx) (t : exp) (T : Typ) : ⊢ Γ ≈ Δ -> Γ ⊢ t : T -> Δ ⊢ t : T
 with
 ctxeq_eq (Γ Δ : Ctx) (t t' : exp) (T : Typ) : ⊢ Γ ≈ Δ -> Γ ⊢ t ≈ t' : T -> Δ ⊢ t ≈ t' : T
@@ -33,13 +35,20 @@ Proof.
     -- pose proof (IHwf_term1 _ H).
        assert (⊢ A :: Γ ≈ A :: Δ) by mauto.
        mauto.
+    -- assert (⊢ ℕ :: Γ ≈ ℕ :: Δ) by (econstructor;mauto).
+       pose proof (IHwf_term1 _ H0).
+       pose proof (IHwf_term2 _ H).
+       assert (⊢ T :: ℕ :: Γ ≈ T :: ℕ :: Δ) by (econstructor;mauto).
+       pose proof (IHwf_term3 _ H3).
+       mauto.
   (*ctxeq_eq*)
   - clear ctxeq_eq.
     intros.
     generalize dependent Δ.
     induction H0.
     1-3: mauto.
-    4-16: mauto.
+    4-6: mauto.
+    10-15,20-23: mauto.
     -- intros.
        pose proof (IHwf_term_eq1 _ H0).
        pose proof (ctxeq_tm _ _ _ _ H0 H).
@@ -51,12 +60,65 @@ Proof.
        eapply wf_eq_conv;mauto.
     -- intros.
        destruct (presup_ctx_eq _ _ H0) as [G D].
-       mauto.       
+       mauto.
+
+    -- intros.
+       assert (⊢ ℕ :: Γ ≈ ℕ :: Δ) by (econstructor;mauto).
+       pose proof (IHwf_term_eq1 _ H1).
+       pose proof (IHwf_term_eq2 _ H0).
+       pose proof (IHwf_term_eq4 _ H0).
+       assert (⊢ T :: ℕ :: Γ ≈ T :: ℕ :: Δ) by (econstructor;mauto).
+       pose proof (IHwf_term_eq3 _ H5).
+       mauto.
+    -- intros.
+       mauto.
+    -- intros.
+       assert (⊢ ℕ :: Γ ≈ ℕ :: Δ) by (econstructor;mauto).
+       pose proof (ctxeq_tm _ _ _ _ H3 H).
+       pose proof (ctxeq_tm _ _ _ _ H2 H0).
+       assert (⊢ T :: ℕ :: Γ ≈ T :: ℕ :: Δ) by (econstructor;mauto).
+       pose proof (ctxeq_tm _ _ _ _ H6 H1).
+       mauto.
+    -- intros.
+       assert (⊢ ℕ :: Γ ≈ ℕ :: Δ) by (econstructor;mauto).
+       pose proof (ctxeq_tm _ _ _ _ H4 H).
+       pose proof (ctxeq_tm _ _ _ _ H3 H0).
+       pose proof (ctxeq_tm _ _ _ _ H3 H2).
+       assert (⊢ T :: ℕ :: Γ ≈ T :: ℕ :: Δ) by (econstructor;mauto).
+       pose proof (ctxeq_tm _ _ _ _ H8 H1).
+       mauto.
+    -- intros.
+       assert (⊢ M :: Γ ≈ M :: Δ) by (econstructor;mauto).
+       pose proof (IHwf_term_eq _ H2).
+       mauto.
+    -- intros.
+       pose proof (IHwf_term_eq1 _ H1).
+       pose proof (IHwf_term_eq2 _ H1).
+       pose proof (ctxeq_tm _ _ _ _ H1 H).
+       assert (⊢ M :: Γ ≈ M :: Δ) by (econstructor;mauto).
+       pose proof (ctxeq_tm _ _ _ _ H5 H0).
+       mauto.
     -- intros.
        inversion H1.
        pose proof (var_in_eq _ _ _ x H4 H0) as [T'' [n [xT'' [GTT'' DTT'']]]].
        destruct (presup_ctx_eq _ _ H4).
        eapply wf_eq_conv;mauto.
+    -- intros.
+       mauto.
+    -- intros.
+       mauto.
+    -- intros.
+       pose proof (ctxeq_tm _ _ _ _ H3 H).
+       assert (⊢ M :: Γ ≈ M :: Δ) by (econstructor;mauto).
+       pose proof (ctxeq_tm _ _ _ _ H5 H0).
+       pose proof (ctxeq_tm _ _ _ _ H5 H1).
+       mauto.
+    -- intros.
+       pose proof (ctxeq_tm _ _ _ _ H2 H).
+       pose proof (ctxeq_tm _ _ _ _ H2 H1).
+       assert (⊢ M :: Γ ≈ M :: Δ) by (econstructor;mauto).
+       pose proof (ctxeq_tm _ _ _ _ H5 H0).
+       mauto.
   (*ctxeq_s*)
   - clear ctxeq_s.
     intros.
@@ -84,7 +146,12 @@ Proof.
        mauto.
     -- pose proof (ctxeq_s _ _ _ _ H H0).
        mauto.
+
+       Unshelve.
+       1-4: exact 0.
 Qed.  
 
+#[export]
+Hint Resolve ctxeq_tm ctxeq_eq ctxeq_s ctxeq_s_eq : mcltt.
 
 
